add Karatsuba's mult to the spec

specs/experimental/Spec.RSA.Bignum.fst
@@ -22,167 +22,253 @@ let bn_is_less x y = x < y
 
 type elem (n:bignum) = e:bignum{bn_v e < bn_v n}
 
-#reset-options "--z3rlimit 150 --max_fuel 0"
+type sign =
+     | Positive : sign
+     | Negative : sign
 
-val mont_reduction:
-	modBits:size_nat{1 < modBits /\ modBits < pow2 32} ->
-	r:nat{r = pow2 (modBits + 2) /\ r > 0} ->
-	n:nat{1 < n /\ 4 * n < r} -> n':bignum ->
-	c:nat{c < r * n} -> Pure (elem (n + n))
-	(requires (True))
-	(ensures (fun res -> res % n == (c / r) % n))
-let mont_reduction modBits r n n' c =
-	let m = (c * n') % r in
-	assert (0 <= m /\ m < r);
-	let m = r - m in
-	assert (0 < m /\ m <= r);
-	let res = (c + n * m) / r in
-	assert (res >= 0);
-	assert (c + n * m <= c + n * r);
-	lemma_div_le (c + n * m) (c + n * r) r;
-	assert (res <= (c + n * r) / r);
-	division_addition_lemma c r n;
-	assert (res <= c / r + n);
-	assert (c / r < n);
-	assert (res < n + n);
-	lemma_mont_reduction res r c n m;
-	res
+(* a - b = (sign, |a - b|) *)
+val abs_sub: 
+    x:size_nat -> a:bignum -> b:bignum -> Pure (tuple2 sign bignum)
+    (requires (a < pow2 (pow2 x) /\ b < pow2 (pow2 x)))
+    (ensures (fun (s, res) -> res < pow2 (pow2 x) /\ res = abs (a - b)))
+    
+let abs_sub x a b =
+    if (bn_is_less a b)
+    then begin
+        assert (b >= a);
+        (Negative, b - a) end
+    else begin
+        assert (a >= b);
+        (Positive, a - b) end
 
-val mul_mod_mont:
-	modBits:size_nat{1 < modBits /\ modBits < pow2 32} ->
-	r:nat{r = pow2 (modBits + 2) /\ r > 0} ->
-	n:nat{1 < n /\ 4 * n < r} -> n':bignum ->
-	a:elem (n + n) -> b:elem (n + n) -> Pure (elem (n + n))
-	(requires (True))
-	(ensures (fun res -> res % n == (a * b / r) % n))
-let mul_mod_mont modBits r n n' a b =
-	let c = a * b in
-	assert (c < 4 * n * n);
-	assert (c < r * n);
- 	mont_reduction modBits r n n' c
+val add_sign:
+    c0:bignum -> c1:bignum -> c2:bignum ->
+    a0:bignum -> a1:bignum -> a2:bignum ->
+    b0:bignum -> b1:bignum -> b2:bignum -> Pure bignum
+    (requires (c0 == a0 * b0 /\ c1 == a1 * b1 /\ c2 == a2 * b2 /\
+               a2 = abs (a0 - a1) /\ b2 = abs (b0 - b1)))
+    (ensures (fun res -> res == a1 * b0 + a0 * b1))
 
-val to_mont:
-	modBits:size_nat{1 < modBits /\ modBits < pow2 32} ->
-	r:nat{r = pow2 (modBits + 2) /\ r > 0} ->
-	n:nat{1 < n /\ 4 * n < r} -> n':bignum ->
-	r2:elem n -> a:elem n -> Pure (elem (n + n))
-	(requires (r2 == (r * r) % n))
-	(ensures (fun res -> res % n == (a * r) % n))
-let to_mont modBits r n n' r2 a =
-	let c = a * r2 in
-	assert (c == a * ((r * r) % n));
-	assert (c < n * n);
-	assert (c < r * n);
-	let res = mont_reduction modBits r n n' c in
-	assert (res % n == ((a * ((r * r) % n)) / r) % n);
-	lemma_mod_div_simplify res a r n;
-	res
+#reset-options "--z3rlimit 150 --initial_fuel 0 --max_fuel 0"
 
-val from_mont:
-	modBits:size_nat{1 < modBits /\ modBits < pow2 32} ->
-	r:nat{r = pow2 (modBits + 2) /\ r > 0} ->
-	n:nat{1 < n /\ 4 * n < r} -> n':bignum ->
-	a_r:elem (n + n) -> Pure (elem n)
-	(requires (True))
-	(ensures (fun res -> res == (a_r / r) % n))
-let from_mont modBits r n n' a_r =
-	let m = (a_r * n') % r in
-	assert (0 <= m /\ m < r);
-	let m = r - m in
-	assert (0 < m /\ m <= r);
-	let res:nat = (a_r + n * m) / r in
-	assert (a_r + n * m <= a_r + n * r);
-	lemma_div_le (a_r + n * m) (a_r + n * r) r;
-	assert (res <= (a_r + n * r) / r);
-	division_addition_lemma a_r r n;
-	assert (res <= a_r / r + n);
-	small_division_lemma_1 a_r r;
-	assert (res <= n);
-	lemma_mont_reduction_1 res r a_r n m;
-	res
+let add_sign c0 c1 c2 a0 a1 a2 b0 b1 b2 =
+    let sa2 = if (a0 >= a1) then Positive else Negative in
+    let sb2 = if (b0 >= b1) then Positive else Negative in
+    if ((sa2 = Positive && sb2 = Positive) || (sa2 = Negative && sb2 = Negative)) 
+    then (c0 + c1) - c2
+    else (c0 + c1) + c2
 
-#reset-options "--z3rlimit 50 --max_fuel 2"
-
-val mont_inverse_:
-	n:bignum -> exp_2:size_nat -> nInv:bignum -> i:size_nat{1 < i /\ i <= exp_2} ->
-	pow2_i1:bignum{0 < pow2_i1} -> pow2_i:bignum -> Tot bignum
-	(decreases (exp_2 - i))
-let rec mont_inverse_ n exp_2 nInv i pow2_i1 pow2_i =
-	if i < exp_2 then begin
-		let pow2_i1 = pow2_i1 * 2 in
-		let pow2_i = pow2_i1 * 2 in
-		let nnInv = (n * nInv) % pow2_i in
-		let nInv = if (pow2_i1 < nnInv) then nInv + pow2_i1 else nInv in
-		mont_inverse_ n exp_2 nInv (i + 1) pow2_i1 pow2_i end
-	else nInv
-
-#reset-options "--z3rlimit 50 --max_fuel 0"
-
-//res = n^(-1) % 2^(exp_2)
-val mont_inverse:
-	n:bignum -> exp_2:size_nat{1 < exp_2 /\ exp_2 + 1 <= max_size_t} -> Tot bignum
-let mont_inverse n exp_2 = mont_inverse_ n (exp_2 + 1) 1 2 1 0
+val karatsuba:
+    x0:size_nat -> a:bignum{a < pow2 (pow2 x0)} -> b:bignum{b < pow2 (pow2 x0)} -> Pure bignum
+    (requires (True))
+    (ensures (fun res -> res == a * b))
+    (decreases x0)
 
 #reset-options "--z3rlimit 150 --max_fuel 2"
 
+let rec karatsuba x0 a b =
+    if x0 < 9 then a * b
+    else begin
+        let x = x0 - 1 in
+        let pow_x = pow2 (pow2 x) in
+	
+        let a0 = a % pow_x in let a1 = a / pow_x in
+        assert (0 <= a0 /\ a0 < pow_x);
+        lemma_pow_div_karatsuba x0 a;
+        assert (0 <= a1 /\ a1 < pow_x);
+        lemma_div_mod a pow_x;
+
+        let b0 = b % pow_x in let b1 = b / pow_x in
+        assert (0 <= b0 /\ b0 < pow_x);
+        lemma_pow_div_karatsuba x0 b;
+        assert (0 <= b1 /\ b1 < pow_x);
+        lemma_div_mod b pow_x;
+
+        let (sa2, a2) = abs_sub x a0 a1 in
+        let (sb2, b2) = abs_sub x b0 b1 in
+		
+        let c0 = karatsuba x a0 b0 in
+        assert (c0 == a0 * b0); //from ind hypo
+        let c1 = karatsuba x a1 b1 in
+        assert (c1 == a1 * b1); //from ind hypo
+        let c2 = karatsuba x a2 b2 in
+        assert (c2 == a2 * b2); //from ind hypo
+		
+        let pow_x1 = pow2 (pow2 (x + 1)) in
+        let tmp = add_sign c0 c1 c2 a0 a1 a2 b0 b1 b2 in
+        let c = c1 * pow_x1 + tmp * pow_x + c0 in
+        lemma_karatsuba_mult x a a0 a1 b b0 b1;
+        assert (c == a * b);
+        c
+    end
+
+val mont_reduction:
+    modBits:size_nat{1 < modBits /\ modBits < pow2 32} ->
+    r:nat{r = pow2 (modBits + 2) /\ r > 0} ->
+    n:nat{1 < n /\ 4 * n < r} -> n':bignum ->
+    c:nat{c < r * n} -> Pure (elem (n + n))
+    (requires (True))
+    (ensures (fun res -> res % n == (c / r) % n))
+
+#reset-options "--z3rlimit 300 --max_fuel 0"
+
+let mont_reduction modBits r n n' c =
+    let m = (c * n') % r in
+    assert (0 <= m /\ m < r);
+    let m = r - m in
+    assert (0 < m /\ m <= r);
+    let res = (c + n * m) / r in
+    assert (res >= 0);
+    assert (c + n * m <= c + n * r);
+    lemma_div_le (c + n * m) (c + n * r) r;
+    assert (res <= (c + n * r) / r);
+    division_addition_lemma c r n;
+    assert (res <= c / r + n);
+    assert (c / r < n);
+    assert (res < n + n);
+    lemma_mont_reduction res r c n m;
+    res
+
+val mul_mod_mont:
+    x0:size_nat ->
+    modBits:size_nat{1 < modBits /\ modBits < pow2 32} ->
+    r:nat{r = pow2 (modBits + 2) /\ r > 0} ->
+    n:nat{1 < n /\ 4 * n < r /\ r <= pow2 (pow2 x0)} -> n':bignum ->
+    a:elem (n + n) -> b:elem (n + n) -> Pure (elem (n + n))
+    (requires (True))
+    (ensures (fun res -> res % n == (a * b / r) % n))
+    
+let mul_mod_mont x0 modBits r n n' a b =
+    let c = karatsuba x0 a b in
+    assert (c < 4 * n * n);
+    assert (c < r * n);
+    mont_reduction modBits r n n' c
+
+val to_mont:
+    modBits:size_nat{1 < modBits /\ modBits < pow2 32} ->
+    r:nat{r = pow2 (modBits + 2) /\ r > 0} ->
+    n:nat{1 < n /\ 4 * n < r} -> n':bignum ->
+    r2:elem n -> a:elem n -> Pure (elem (n + n))
+    (requires (r2 == (r * r) % n))
+    (ensures (fun res -> res % n == (a * r) % n))
+    
+let to_mont modBits r n n' r2 a =
+    let c = a * r2 in
+    assert (c == a * ((r * r) % n));
+    assert (c < n * n);
+    assert (c < r * n);
+    let res = mont_reduction modBits r n n' c in
+    assert (res % n == ((a * ((r * r) % n)) / r) % n);
+    lemma_mod_div_simplify res a r n;
+    res
+
+val from_mont:
+    modBits:size_nat{1 < modBits /\ modBits < pow2 32} ->
+    r:nat{r = pow2 (modBits + 2) /\ r > 0} ->
+    n:nat{1 < n /\ 4 * n < r} -> n':bignum ->
+    a_r:elem (n + n) -> Pure (elem n)
+    (requires (True))
+    (ensures (fun res -> res == (a_r / r) % n))
+    
+let from_mont modBits r n n' a_r =
+    let m = (a_r * n') % r in
+    assert (0 <= m /\ m < r);
+    let m = r - m in
+    assert (0 < m /\ m <= r);
+    let res:nat = (a_r + n * m) / r in
+    assert (a_r + n * m <= a_r + n * r);
+    lemma_div_le (a_r + n * m) (a_r + n * r) r;
+    assert (res <= (a_r + n * r) / r);
+    division_addition_lemma a_r r n;
+    assert (res <= a_r / r + n);
+    small_division_lemma_1 a_r r;
+    assert (res <= n);
+    lemma_mont_reduction_1 res r a_r n m;
+    res
+
+val mont_inverse_:
+    n:bignum -> exp_2:size_nat -> nInv:bignum -> i:size_nat{1 < i /\ i <= exp_2} ->
+    pow2_i1:bignum{0 < pow2_i1} -> pow2_i:bignum -> Tot bignum
+    (decreases (exp_2 - i))
+
+#reset-options "--z3rlimit 50 --max_fuel 2"
+
+let rec mont_inverse_ n exp_2 nInv i pow2_i1 pow2_i =
+    if i < exp_2 then begin
+        let pow2_i1 = pow2_i1 * 2 in
+        let pow2_i = pow2_i1 * 2 in
+        let nnInv = (n * nInv) % pow2_i in
+        let nInv = if (pow2_i1 < nnInv) then nInv + pow2_i1 else nInv in
+        mont_inverse_ n exp_2 nInv (i + 1) pow2_i1 pow2_i end
+    else nInv
+
+//res = n^(-1) % 2^(exp_2)
+val mont_inverse: n:bignum -> exp_2:size_nat{1 < exp_2 /\ exp_2 + 1 <= max_size_t} -> Tot bignum
+let mont_inverse n exp_2 = mont_inverse_ n (exp_2 + 1) 1 2 1 0
+
+
 val mod_exp_:
-	modBits:size_nat{1 < modBits /\ modBits < pow2 32} ->
-	r:nat{r = pow2 (modBits + 2) /\ r > 0} ->
-	n:nat{1 < n /\ 4 * n < r} -> n':bignum ->
-	a:elem (n + n) -> b:nat -> acc:elem (n + n) -> Pure (elem (n + n))
-	(requires True)
-	(ensures (fun res -> res % n == ((pow a b) * acc / pow r b) % n))
-	(decreases b)
-let rec mod_exp_ modBits r n n' a b acc =
-	if b = 0
-	then acc
-	else begin
-		let a2 = mul_mod_mont modBits r n n' a a in
-		let b2 = bn_div2 b in
-		lemma_div_mod b 2;
-		if (bn_is_even b) then begin
-			assert (b = 2 * b2);
-			let res = mod_exp_ modBits r n n' a2 b2 acc in
-			assert (res % n == ((pow a2 b2) * acc / pow r b2) % n); //from ind hypo
-			lemma_mod_exp n a a2 b b2 acc r res;
-			res end
-		else begin
-			assert (b = 2 * b2 + 1);
-			let acc' = mul_mod_mont modBits r n n' a acc in
-			let res = mod_exp_ modBits r n n' a2 b2 acc' in
-			assert (res % n == ((pow a2 b2) * acc' / pow r b2) % n); //from ind hypo
-			lemma_mod_exp_1 n a a2 b b2 acc acc' r res;
-			res end
-		end
+    x0:size_nat ->
+    modBits:size_nat{1 < modBits /\ modBits < pow2 32} ->
+    r:nat{r = pow2 (modBits + 2) /\ r > 0} ->
+    n:nat{1 < n /\ 4 * n < r /\ r < pow2 (pow2 x0)} -> n':bignum ->
+    a:elem (n + n) -> b:nat -> acc:elem (n + n) -> Pure (elem (n + n))
+    (requires True)
+    (ensures (fun res -> res % n == ((pow a b) * acc / pow r b) % n))
+    (decreases b)
+
+#reset-options "--z3rlimit 150 --max_fuel 2"
+
+let rec mod_exp_ x0 modBits r n n' a b acc =
+    if b = 0
+    then acc
+    else begin
+        let a2 = mul_mod_mont x0 modBits r n n' a a in
+        let b2 = bn_div2 b in
+        lemma_div_mod b 2;
+        if (bn_is_even b) then begin
+            assert (b = 2 * b2);
+            let res = mod_exp_ x0 modBits r n n' a2 b2 acc in
+            assert (res % n == ((pow a2 b2) * acc / pow r b2) % n); //from ind hypo
+            lemma_mod_exp n a a2 b b2 acc r res;
+            res end
+        else begin
+            assert (b = 2 * b2 + 1);
+            let acc' = mul_mod_mont x0 modBits r n n' a acc in
+            let res = mod_exp_ x0 modBits r n n' a2 b2 acc' in
+            assert (res % n == ((pow a2 b2) * acc' / pow r b2) % n); //from ind hypo
+            lemma_mod_exp_1 n a a2 b b2 acc acc' r res;
+            res end
+        end
+
+val mod_exp:
+    x0:size_nat ->
+    modBits:size_nat{1 < modBits /\ modBits + 3 < pow2 32} ->
+    n:bignum{1 < n /\ n < pow2 modBits /\ pow2 (modBits + 2) < pow2 (pow2 x0)} ->
+    a:elem n -> b:bignum -> Pure (elem n)
+    (requires True)
+    (ensures (fun res -> res == (pow a b) % n))
 
 #reset-options "--z3rlimit 150 --max_fuel 0"
 
-val mod_exp:
-	modBits:size_nat{1 < modBits /\ modBits + 3 < pow2 32} ->
-	n:bignum{1 < n /\ n < pow2 modBits} ->
-	a:elem n -> b:bignum -> Pure (elem n)
-	(requires True)
-	(ensures (fun res -> res == (pow a b) % n))
-let mod_exp modBits n a b =
-	let r = pow2 (2 + modBits) in
-	lemma_r_n modBits r n;
-	let n'= mont_inverse n (2 + modBits) in
-	let r2 = (r * r) % n in
-	let a_r = to_mont modBits r n n' r2 a in
-	let acc_r = to_mont modBits r n n' r2 1 in
-	let res_r = mod_exp_ modBits r n n' a_r b acc_r in
-	lemma_mod_exp_2 n a a_r b acc_r r res_r;
-	let res = from_mont modBits r n n' res_r in
-	lemma_mod_mult_div_1 res_r r n;
-	lemma_mod_mult_div_1 ((pow a b) * r) r n;
-	multiple_division_lemma (pow a b) r;
-	res
+let mod_exp x0 modBits n a b =
+    let r = pow2 (2 + modBits) in
+    lemma_r_n modBits r n;
+    let n'= mont_inverse n (2 + modBits) in
+    let r2 = (r * r) % n in
+    let a_r = to_mont modBits r n n' r2 a in
+    let acc_r = to_mont modBits r n n' r2 1 in
+    let res_r = mod_exp_ x0 modBits r n n' a_r b acc_r in
+    lemma_mod_exp_2 n a a_r b acc_r r res_r;
+    let res = from_mont modBits r n n' res_r in
+    lemma_mod_mult_div_1 res_r r n;
+    lemma_mod_mult_div_1 ((pow a b) * r) r n;
+    multiple_division_lemma (pow a b) r;
+    res
 
 (* BIGNUM CONVERT FUNCTIONS *)
-val os2ip:
-	bLen:size_nat{bLen > 0} -> b:lbytes bLen -> Tot (res:bignum{bn_v res < pow2 (8 * bLen)})
+val os2ip:bLen:size_nat{bLen > 0} -> b:lbytes bLen -> Tot (res:bignum{res < pow2 (8 * bLen)})
 let os2ip bLen b = nat_from_intseq_be #U8 #bLen b
 
-val i2osp:
-	n:bignum -> bLen:size_nat{bn_v n < pow2 (8 * bLen)} -> b:lbytes bLen -> Tot (lbytes bLen)
+val i2osp:n:bignum -> bLen:size_nat{n < pow2 (8 * bLen)} -> b:lbytes bLen -> Tot (lbytes bLen)
 let i2osp n bLen b = nat_to_bytes_be bLen n
