specs/experimental/Spec.RSA.fst
@@ -26,264 +26,267 @@ let eq_bytes len b1 b2 = for_all2 (fun x y -> uint_to_nat #U8 x = uint_to_nat #U
 let max_input_len_sha256 = pow2 61
 unfold let hLen = 32
 val hash_sha256:
-	msgLen:size_nat{msgLen < max_input_len_sha256} ->
-	msg:lbytes msgLen ->
-	hash:lbytes hLen ->
-	Tot (msgHash:lbytes hLen)
+    msgLen:size_nat{msgLen < max_input_len_sha256} ->
+    msg:lbytes msgLen ->
+    hash:lbytes hLen ->
+    Tot (msgHash:lbytes hLen)
 let hash_sha256 msgLen msg hash = Hash.hash256 msgLen msg
 
 (* Mask Generation Function *)
 val mgf_sha256_loop:
-	mgfseedLen:size_nat{mgfseedLen = hLen + 4 /\ mgfseedLen < max_input_len_sha256} ->
-	mgfseed:lbytes mgfseedLen ->
+    mgfseedLen:size_nat{mgfseedLen = hLen + 4 /\ mgfseedLen < max_input_len_sha256} ->
+    mgfseed:lbytes mgfseedLen ->
     counter_max:size_nat{counter_max * hLen < pow2 32}->
-	accLen:size_nat{accLen = counter_max * hLen} ->
-	acc:lbytes accLen ->
-	Tot (res:lbytes accLen)
+    accLen:size_nat{accLen = counter_max * hLen} ->
+    acc:lbytes accLen ->
+    Tot (res:lbytes accLen)
 
 #reset-options "--z3rlimit 30 --max_fuel 0 --max_ifuel 0"
 
 let mgf_sha256_loop mgfseedLen mgfseed counter_max accLen acc =
     let mHash = create hLen (u8 0) in
     let next (i:size_nat{i < counter_max}) (acc:lbytes accLen) : lbytes accLen =
-		let counter = nat_to_bytes_be 4 i in
-		let mgfseed = update_sub mgfseed hLen 4 counter in
-		let mHash = hash_sha256 mgfseedLen mgfseed mHash in
-		update_sub acc (hLen * i) hLen mHash in
+        let counter = nat_to_bytes_be 4 i in
+        let mgfseed = update_sub mgfseed hLen 4 counter in
+        let mHash = hash_sha256 mgfseedLen mgfseed mHash in
+        update_sub acc (hLen * i) hLen mHash in
     repeati #(lbytes accLen) counter_max next acc
-
-#reset-options "--z3rlimit 50 --max_fuel 0"
 
 (* We only allow U32.t masklen, this means that we always have the property
    that maskLen <= op_Multiply (pow2 32) (U32.v hLen) as required by the spec *)
 val mgf_sha256:
-	mgfseedLen:size_nat{mgfseedLen = hLen + 4 /\ mgfseedLen < max_input_len_sha256} ->
-	mgfseed:lbytes mgfseedLen ->
-	maskLen:size_nat{maskLen > 0 /\ (blocks maskLen hLen) * hLen < pow2 32} ->
-	mask:lbytes maskLen ->
-	Tot (mask':lbytes maskLen)
+    mgfseedLen:size_nat{mgfseedLen = hLen + 4 /\ mgfseedLen < max_input_len_sha256} ->
+    mgfseed:lbytes mgfseedLen ->
+    maskLen:size_nat{maskLen > 0 /\ (blocks maskLen hLen) * hLen < pow2 32} ->
+    mask:lbytes maskLen ->
+    Tot (mask':lbytes maskLen)
+
+#reset-options "--z3rlimit 50 --max_fuel 0"
 
 let mgf_sha256 mgfseedLen mgfseed maskLen mask =
-	let counter_max = blocks maskLen hLen in
-	let accLen : size_nat = counter_max * hLen in
-	let acc = create accLen (u8 0) in
-	let acc = mgf_sha256_loop mgfseedLen mgfseed counter_max accLen acc in
-	slice acc 0 maskLen
+    let counter_max = blocks maskLen hLen in
+    let accLen : size_nat = counter_max * hLen in
+    let acc = create accLen (u8 0) in
+    let acc = mgf_sha256_loop mgfseedLen mgfseed counter_max accLen acc in
+    slice acc 0 maskLen
 
 (* RSA *)
 type modBits = modBits:size_nat{1 < modBits /\ modBits + 3 < pow2 32}
 
 noeq type rsa_pubkey (modBits:modBits) =
-	| Mk_rsa_pubkey: n:bignum{1 < n /\ pow2 (modBits - 1) <= bn_v n /\ bn_v n < pow2 modBits} ->
-					 e:elem n{bn_v e > 1} -> rsa_pubkey modBits
+     | Mk_rsa_pubkey: n:bignum{1 < n /\ pow2 (modBits - 1) <= n /\ n < pow2 modBits} ->
+                      e:elem n{1 < e} -> rsa_pubkey modBits
 	
 noeq type rsa_privkey (modBits:modBits) =
-	| Mk_rsa_privkey: pkey:rsa_pubkey modBits ->
-					  d:elem (Mk_rsa_pubkey?.n pkey){bn_v d > 1} ->
-					  p:elem (Mk_rsa_pubkey?.n pkey){bn_v p > 1} ->
-					  q:elem (Mk_rsa_pubkey?.n pkey){bn_v q > 1 /\ bn_v (Mk_rsa_pubkey?.n pkey) = bn_v p * bn_v q} -> rsa_privkey modBits
+     | Mk_rsa_privkey: pkey:rsa_pubkey modBits ->
+                       d:elem (Mk_rsa_pubkey?.n pkey){1 < d} ->
+                       p:elem (Mk_rsa_pubkey?.n pkey){1 < p} ->
+                       q:elem (Mk_rsa_pubkey?.n pkey){1 < q /\ (Mk_rsa_pubkey?.n pkey) = p * q} -> rsa_privkey modBits
 
 val pss_encode_:
-	sLen:size_nat{sLen + hLen + 8 < pow2 32 /\ sLen + hLen + 8 < max_input_len_sha256} ->
-	salt:lbytes sLen ->
-	msgLen:size_nat{msgLen < max_input_len_sha256} ->
-	msg:lbytes msgLen ->
-	emLen:size_nat{0 <= emLen - sLen - hLen - 2 /\ emLen < pow2 32} ->
-	em:lbytes emLen ->
-	Tot (em':lbytes emLen)
+    sLen:size_nat{sLen + hLen + 8 < pow2 32 /\ sLen + hLen + 8 < max_input_len_sha256} ->
+    salt:lbytes sLen ->
+    msgLen:size_nat{msgLen < max_input_len_sha256} ->
+    msg:lbytes msgLen ->
+    emLen:size_nat{0 <= emLen - sLen - hLen - 2 /\ emLen < pow2 32} ->
+    em:lbytes emLen ->
+    Tot (em':lbytes emLen)
 
 let pss_encode_ sLen salt msgLen msg emLen em =
-	let mHash = create hLen (u8 0) in
-	let mHash = hash_sha256 msgLen msg mHash in
+    let mHash = create hLen (u8 0) in
+    let mHash = hash_sha256 msgLen msg mHash in
 
-	let m1_size : size_nat = 8 + hLen + sLen in
-	let m1 = create m1_size (u8 0) in
-	let m1 = update_sub m1 8 hLen mHash in
-	let m1 = update_sub m1 (8 + hLen) sLen salt in
-	let m1Hash = create 36 (u8 0) in
-	let m1Hash' = sub m1Hash 0 hLen in
-	let m1Hash' = hash_sha256 m1_size m1 m1Hash' in
-	let m1Hash = update_sub m1Hash 0 hLen m1Hash' in
+    let m1_size : size_nat = 8 + hLen + sLen in
+    let m1 = create m1_size (u8 0) in
+    let m1 = update_sub m1 8 hLen mHash in
+    let m1 = update_sub m1 (8 + hLen) sLen salt in
+    let m1Hash = create 36 (u8 0) in
+    let m1Hash' = sub m1Hash 0 hLen in
+    let m1Hash' = hash_sha256 m1_size m1 m1Hash' in
+    let m1Hash = update_sub m1Hash 0 hLen m1Hash' in
 
-	let db_size : size_nat = emLen - hLen - 1 in
-	let db = create db_size (u8 0) in
-	let last_before_salt = db_size - sLen - 1 in
-	let db = db.[last_before_salt] <- (u8 1) in
-	let db = update_sub db (last_before_salt + 1) sLen salt in
+    let db_size : size_nat = emLen - hLen - 1 in
+    let db = create db_size (u8 0) in
+    let last_before_salt = db_size - sLen - 1 in
+    let db = db.[last_before_salt] <- (u8 1) in
+    let db = update_sub db (last_before_salt + 1) sLen salt in
 
     let dbMask = create db_size (u8 0) in
-	let dbMask = mgf_sha256 (hLen + 4) m1Hash db_size dbMask in
-	let maskedDB = xor_bytes db_size db dbMask in
-	let em = update_sub em 0 db_size maskedDB in
-	let em = update_sub em db_size hLen m1Hash' in
-	em.[emLen - 1] <- (u8 188)
+    let dbMask = mgf_sha256 (hLen + 4) m1Hash db_size dbMask in
+    let maskedDB = xor_bytes db_size db dbMask in
+    let em = update_sub em 0 db_size maskedDB in
+    let em = update_sub em db_size hLen m1Hash' in
+    em.[emLen - 1] <- (u8 188)
 
 val pss_encode:
-	msBits:size_nat{msBits < 8} ->
-	sLen:size_nat{sLen + hLen + 8 < pow2 32 /\ sLen + hLen + 8 < max_input_len_sha256} ->
-	salt:lbytes sLen ->
-	msgLen:size_nat{msgLen < max_input_len_sha256} ->
-	msg:lbytes msgLen ->
-	emLen:size_nat{0 <= emLen - sLen - hLen - 3 /\ emLen < pow2 32} ->
-	em:lbytes emLen ->
-	Tot (lbytes emLen)
+    msBits:size_nat{msBits < 8} ->
+    sLen:size_nat{sLen + hLen + 8 < pow2 32 /\ sLen + hLen + 8 < max_input_len_sha256} ->
+    salt:lbytes sLen ->
+    msgLen:size_nat{msgLen < max_input_len_sha256} ->
+    msg:lbytes msgLen ->
+    emLen:size_nat{0 <= emLen - sLen - hLen - 3 /\ emLen < pow2 32} ->
+    em:lbytes emLen ->
+    Tot (lbytes emLen)
 
 let pss_encode msBits sLen salt msgLen msg emLen em =
-	if msBits = 0
-	then begin
-		let em' = sub em 1 (emLen - 1) in
-		let em' = pss_encode_ sLen salt msgLen msg (emLen - 1) em' in
-		update_sub em 1 (emLen - 1) em' end
-	else begin
-		let em = pss_encode_ sLen salt msgLen msg emLen em in
-		assert (0 < 8 - msBits /\ 8 - msBits < 8);
-		em.[0] <- em.[0] &. ((u8 255) >>. u32 (8 - msBits)) end
+    if msBits = 0
+    then begin
+        let em' = sub em 1 (emLen - 1) in
+        let em' = pss_encode_ sLen salt msgLen msg (emLen - 1) em' in
+        update_sub em 1 (emLen - 1) em' end
+    else begin
+        let em = pss_encode_ sLen salt msgLen msg emLen em in
+        assert (0 < 8 - msBits /\ 8 - msBits < 8);
+        em.[0] <- em.[0] &. ((u8 255) >>. u32 (8 - msBits)) end
 
 val pss_verify_:
-	sLen:size_nat{sLen + hLen + 8 < pow2 32 /\ sLen + hLen + 8 < max_input_len_sha256} ->
-	msBits:size_nat{msBits < 8} ->
-	emLen:size_nat{0 <= emLen - sLen - hLen - 2 /\ emLen < pow2 32} ->
-	em:lbytes emLen ->
-	msgLen:size_nat{msgLen < max_input_len_sha256} ->
-	msg:lbytes msgLen -> Tot bool
+    sLen:size_nat{sLen + hLen + 8 < pow2 32 /\ sLen + hLen + 8 < max_input_len_sha256} ->
+    msBits:size_nat{msBits < 8} ->
+    emLen:size_nat{0 <= emLen - sLen - hLen - 2 /\ emLen < pow2 32} ->
+    em:lbytes emLen ->
+    msgLen:size_nat{msgLen < max_input_len_sha256} ->
+    msg:lbytes msgLen -> Tot bool
 
 let pss_verify_ sLen msBits emLen em msgLen msg =
-	let mHash = create hLen (u8 0) in
-	let mHash = hash_sha256 msgLen msg mHash in
+    let mHash = create hLen (u8 0) in
+    let mHash = hash_sha256 msgLen msg mHash in
 
-	let (pad_size:size_nat{pad_size > 0}) = emLen - sLen - hLen - 1 in
-	let pad2 = create pad_size (u8 0) in
-	let pad2 = pad2.[pad_size - 1] <- (u8 1) in
+    let (pad_size:size_nat{pad_size > 0}) = emLen - sLen - hLen - 1 in
+    let pad2 = create pad_size (u8 0) in
+    let pad2 = pad2.[pad_size - 1] <- (u8 1) in
 
-	let (db_size:size_nat{db_size > 0}) = emLen - hLen - 1 in
-	let maskedDB = slice em 0 db_size in
-	let m1Hash0 = slice em db_size (db_size + hLen) in
-	let m1Hash = create 36 (u8 0) in
-	let m1Hash = update_sub m1Hash 0 hLen m1Hash0 in
-	let dbMask = create db_size (u8 0) in
-	let dbMask = mgf_sha256 (hLen + 4) m1Hash db_size dbMask in
-	let db = xor_bytes db_size maskedDB dbMask in
-	let db =
-		if msBits > 0
-		then begin
-			assert (0 < 8 - msBits /\ 8 - msBits < 8);
-			db.[0] <- db.[0] &. (u8 255 >>. u32 (8 - msBits)) end
-		else db in
+    let (db_size:size_nat{db_size > 0}) = emLen - hLen - 1 in
+    let maskedDB = slice em 0 db_size in
+    let m1Hash0 = slice em db_size (db_size + hLen) in
+    let m1Hash = create 36 (u8 0) in
+    let m1Hash = update_sub m1Hash 0 hLen m1Hash0 in
+    let dbMask = create db_size (u8 0) in
+    let dbMask = mgf_sha256 (hLen + 4) m1Hash db_size dbMask in
+    let db = xor_bytes db_size maskedDB dbMask in
+    let db =
+        if msBits > 0
+        then begin
+            assert (0 < 8 - msBits /\ 8 - msBits < 8);
+            db.[0] <- db.[0] &. (u8 255 >>. u32 (8 - msBits)) end
+        else db in
 	
-	let pad = slice db 0 pad_size in
-	let salt = slice db pad_size (pad_size + sLen) in
+    let pad = slice db 0 pad_size in
+    let salt = slice db pad_size (pad_size + sLen) in
 
-	let m1_size:size_nat = 8 + hLen + sLen in
-	let m1 = create m1_size (u8 0) in
-	let m1Hash' = create hLen (u8 0) in
-	if not (eq_bytes pad_size pad pad2) then false
-	else begin
-		(* first 8 elements should be 0x00 *)
-		let m1 = update_sub m1 8 hLen mHash in
-		let m1 = update_sub m1 (8 + hLen) sLen salt in
-		let m1Hash' = hash_sha256 m1_size m1 m1Hash' in
-		eq_bytes hLen m1Hash0 m1Hash'
-	end
+    let m1_size:size_nat = 8 + hLen + sLen in
+    let m1 = create m1_size (u8 0) in
+    let m1Hash' = create hLen (u8 0) in
+    if not (eq_bytes pad_size pad pad2) then false
+    else begin
+        (* first 8 elements should be 0x00 *)
+        let m1 = update_sub m1 8 hLen mHash in
+        let m1 = update_sub m1 (8 + hLen) sLen salt in
+        let m1Hash' = hash_sha256 m1_size m1 m1Hash' in
+        eq_bytes hLen m1Hash0 m1Hash'
+    end
 
 val pss_verify:
-	sLen:size_nat{sLen + hLen + 8 < pow2 32 /\ sLen + hLen + 8 < max_input_len_sha256} ->
-	msBits:size_nat{msBits < 8} ->
-	emLen:size_nat{0 < emLen /\ emLen < pow2 32} ->
-	em:lbytes emLen ->
-	msgLen:size_nat{msgLen < max_input_len_sha256} ->
-	msg:lbytes msgLen -> Tot bool
+    sLen:size_nat{sLen + hLen + 8 < pow2 32 /\ sLen + hLen + 8 < max_input_len_sha256} ->
+    msBits:size_nat{msBits < 8} ->
+    emLen:size_nat{0 < emLen /\ emLen < pow2 32} ->
+    em:lbytes emLen ->
+    msgLen:size_nat{msgLen < max_input_len_sha256} ->
+    msg:lbytes msgLen -> Tot bool
 
 let pss_verify sLen msBits emLen em msgLen msg =
-	let em_0 = em.[0] &. (u8 255 <<. u32 msBits) in
-	let em_last = em.[emLen - 1] in
+    let em_0 = em.[0] &. (u8 255 <<. u32 msBits) in
+    let em_last = em.[emLen - 1] in
 
-	if not ((uint_to_nat #U8 em_0 = 0) && (uint_to_nat #U8 em_last = 188))
-	then false
-	else begin
-		let emLen' = if msBits = 0 then emLen - 1 else emLen in
-		let em':lbytes emLen' = if msBits = 0 then sub em 1 (emLen - 1) else em in
-		if (emLen' < sLen + hLen + 2)
-		then false
-		else pss_verify_ sLen msBits emLen' em' msgLen msg
-		end
+    if not ((uint_to_nat #U8 em_0 = 0) && (uint_to_nat #U8 em_last = 188))
+    then false
+    else begin
+        let emLen' = if msBits = 0 then emLen - 1 else emLen in
+        let em':lbytes emLen' = if msBits = 0 then sub em 1 (emLen - 1) else em in
+        if (emLen' < sLen + hLen + 2)
+        then false
+        else pss_verify_ sLen msBits emLen' em' msgLen msg
+    end
 
 val rsa_blinding:
-	modBits:modBits ->
-	n:bignum{1 < n /\ n < pow2 modBits} ->
-	p:elem n{1 < p} ->
-	q:elem n{1 < q /\ n = p * q} ->
-	d:elem n{1 < d} ->
-	m:elem n ->
-	rBlind:bignum{rBlind < pow2 64} -> Tot (s:bignum{s == (pow m d) % n})
+    x0:size_nat ->
+    modBits:modBits ->
+    n:bignum{1 < n /\ n < pow2 modBits /\ pow2 (modBits + 2) < pow2 (pow2 x0)} ->
+    p:elem n{1 < p} ->
+    q:elem n{1 < q /\ n = p * q} ->
+    d:elem n{1 < d} ->
+    m:elem n ->
+    rBlind:bignum{rBlind < pow2 64} -> Tot (s:bignum{s == (pow m d) % n})
 
-let rsa_blinding modBits n p q d m rBlind =
-	let phi_n:nat = (p - 1) * (q - 1) in
-	let d':nat = d + rBlind * phi_n in
-	let s = mod_exp modBits n m d' in
-	assert (s == (pow m d') % n);
-	lemma_exp_blinding n phi_n p q d m rBlind;
-	assert (s == (pow m d) % n);
-	s
+let rsa_blinding x0 modBits n p q d m rBlind =
+    let phi_n:nat = (p - 1) * (q - 1) in
+    let d':nat = d + rBlind * phi_n in
+    let s = mod_exp x0 modBits n m d' in
+    assert (s == (pow m d') % n);
+    lemma_exp_blinding n phi_n p q d m rBlind;
+    assert (s == (pow m d) % n);
+    s
 
 val rsa_sign:
-	modBits:modBits ->
-	skey:rsa_privkey modBits ->
-	rBlind:bignum{rBlind < pow2 64} ->
-	sLen:size_nat{sLen + hLen + 8 < pow2 32 /\ 0 <= (blocks modBits 8) - sLen - hLen - 3 /\
-				  sLen + hLen + 8 < max_input_len_sha256} ->
-	salt:lbytes sLen ->
-	msgLen:size_nat{msgLen < max_input_len_sha256} ->
-	msg:lbytes msgLen ->
-	Tot (sgnt:lbytes (blocks modBits 8))
+    x0:size_nat ->
+    modBits:modBits{pow2 (modBits + 2) < pow2 (pow2 x0)} ->
+    skey:rsa_privkey modBits ->
+    rBlind:bignum{rBlind < pow2 64} ->
+    sLen:size_nat{sLen + hLen + 8 < pow2 32 /\ 0 <= (blocks modBits 8) - sLen - hLen - 3 /\
+                  sLen + hLen + 8 < max_input_len_sha256} ->
+    salt:lbytes sLen ->
+    msgLen:size_nat{msgLen < max_input_len_sha256} ->
+    msg:lbytes msgLen ->
+    Tot (sgnt:lbytes (blocks modBits 8))
 
-let rsa_sign modBits skey rBlind sLen salt msgLen msg =
-	let pkey = Mk_rsa_privkey?.pkey skey in
-	let n = Mk_rsa_pubkey?.n pkey in
-	let e = Mk_rsa_pubkey?.e pkey in
-	let d = Mk_rsa_privkey?.d skey in
-	let p = Mk_rsa_privkey?.p skey in
-	let q = Mk_rsa_privkey?.q skey in
-	let k = blocks modBits 8 in
-	assert (modBits <= 8 * k);
-	pow2_le_compat (8 * k) modBits;
-	assert (pow2 modBits <= pow2 (8 * k));
-	assert (bn_v n < pow2 (8 * k));
+let rsa_sign x0 modBits skey rBlind sLen salt msgLen msg =
+    let pkey = Mk_rsa_privkey?.pkey skey in
+    let n = Mk_rsa_pubkey?.n pkey in
+    let e = Mk_rsa_pubkey?.e pkey in
+    let d = Mk_rsa_privkey?.d skey in
+    let p = Mk_rsa_privkey?.p skey in
+    let q = Mk_rsa_privkey?.q skey in
+    let k = blocks modBits 8 in
+    assert (modBits <= 8 * k);
+    pow2_le_compat (8 * k) modBits;
+    assert (pow2 modBits <= pow2 (8 * k));
+    assert (n < pow2 (8 * k));
 	
-	let msBits = (modBits - 1) % 8 in
-	let em = create k (u8 0) in
-	let em = pss_encode msBits sLen salt msgLen msg k em in
-	let m = os2ip k em in
+    let msBits = (modBits - 1) % 8 in
+    let em = create k (u8 0) in
+    let em = pss_encode msBits sLen salt msgLen msg k em in
+    let m = os2ip k em in
 	
-	assume (bn_v m < bn_v n);
-	let s = rsa_blinding modBits n p q d m rBlind in
+    assume (m < n);
+    let s = rsa_blinding x0 modBits n p q d m rBlind in
 
-	let sgnt = create k (u8 0) in
-	assert (bn_v s < bn_v n);
-	i2osp s k sgnt
+    let sgnt = create k (u8 0) in
+    assert (s < n);
+    i2osp s k sgnt
 
 val rsa_verify:
-	modBits:modBits ->
-	pkey:rsa_pubkey modBits ->
-	sLen:size_nat{sLen + hLen + 8 < pow2 32 /\ sLen + hLen + 8 < max_input_len_sha256} ->
-	sgnt:lbytes (blocks modBits 8) ->
-	msgLen:size_nat{msgLen < max_input_len_sha256} ->
-	msg:lbytes msgLen -> Tot bool
+    x0:size_nat ->
+    modBits:modBits{pow2 (modBits + 2) < pow2 (pow2 x0)} ->
+    pkey:rsa_pubkey modBits ->
+    sLen:size_nat{sLen + hLen + 8 < pow2 32 /\ sLen + hLen + 8 < max_input_len_sha256} ->
+    sgnt:lbytes (blocks modBits 8) ->
+    msgLen:size_nat{msgLen < max_input_len_sha256} ->
+    msg:lbytes msgLen -> Tot bool
 
-let rsa_verify modBits pkey sLen sgnt msgLen msg =
-	let n = Mk_rsa_pubkey?.n pkey in
-	let e = Mk_rsa_pubkey?.e pkey in
-	let k = blocks modBits 8 in
-	assert (modBits <= 8 * k);
-	pow2_le_compat (8 * k) modBits;
-	assert (pow2 modBits <= pow2 (8 * k));
-	assert (n < pow2 (8 * k));
+let rsa_verify x0 modBits pkey sLen sgnt msgLen msg =
+    let n = Mk_rsa_pubkey?.n pkey in
+    let e = Mk_rsa_pubkey?.e pkey in
+    let k = blocks modBits 8 in
+    assert (modBits <= 8 * k);
+    pow2_le_compat (8 * k) modBits;
+    assert (pow2 modBits <= pow2 (8 * k));
+    assert (n < pow2 (8 * k));
 
-	let s = os2ip k sgnt in
-	if bn_is_less s n then begin
-		assert (bn_v s < bn_v n);
-		let m = mod_exp modBits n s e in
-		let em = create k (u8 0) in
-		let em = i2osp m k em in
-		let msBits = (modBits - 1) % 8 in
-		pss_verify sLen msBits k em msgLen msg end
-	else false
+    let s = os2ip k sgnt in
+    if bn_is_less s n then begin
+        assert (s < n);
+        let m = mod_exp x0 modBits n s e in
+        let em = create k (u8 0) in
+        let em = i2osp m k em in
+        let msBits = (modBits - 1) % 8 in
+        pss_verify sLen msBits k em msgLen msg end
+    else false
